Try out rely guarantee reasoning (not sure about the correctness yet!)

examples/locks/Locks.hs
@@ -13,3 +13,17 @@ deadlock = do
   m <- newEmptyMVar :: IO (MVar Int)
   x <- takeMVar m
   return ()
+
+t1 :: MVar Int -> MVar Int -> IO ()
+t1 bal cost = do
+  modifyMVar_ bal $ \x -> return (x + 5000)
+  modifyMVar_ bal $ \x -> return (x + 1000)
+  modifyMVar_ bal $ \x -> return (x * 2)
+  return ()
+
+t2 :: MVar Int -> MVar Int -> IO ()
+t2 bal cost = do
+  x <- readMVar bal
+  if (x >= 1000) then
+    do putMVar cost 100
+  else do putMVar cost 0
