examples/locks/Proofs.v
@@ -5,6 +5,8 @@ Require Import Proofs.Control.Concurrency.Interp.
 
 Require Import Locks.
 
+Require Import Psatz.
+
 Axiom decode_encode_word : forall (w : Word),
     decode (encode w) = Some w.
 
@@ -30,4 +32,104 @@ Qed.
 Theorem deadlock_prog_unsafe : ~ safe_single_prog deadlock.
 Proof.
   apply deadlock_unsafe. apply deadlock_prog_deadlock.
+Qed.
+
+Require Import ZArith.
+
+Open Scope Z_scope.
+
+Axiom decode_encode_int : forall (w : Int),
+    decode (encode w) = Some w.
+
+Definition access_heap { A } (h : heap) (loc : GHC.Num.Word) : option A :=
+  match content h loc with
+  | Some w => decode w
+  | None => None
+  end.
+
+Definition R1 bloc : rely :=
+  fun h1 h2 =>
+    @access_heap Int h1 bloc = access_heap h2 bloc.
+
+Definition G1 bloc : guarantee :=
+  fun h1 h2 =>
+    forall bal,
+      access_heap h2 bloc = Some bal ->
+      bal >= 1000.
+
+Ltac prove_guarantee :=
+  let H := fresh "H" in
+  intros ? H; unfold access_heap in H; simpl in H;
+  rewrite N.eqb_refl in H;
+  first [rewrite decode_encode_int in H; inversion H; lia |
+         discriminate].
+
+Ltac split_g :=
+  split; [| prove_guarantee].
+
+Ltac destruct_match :=
+  match goal with
+  | |- context[match ?a with _ => _ end] =>
+    let Hm := fresh "Hmatch" in
+    destruct a eqn:Hm
+  end.
+
+Ltac use_rely Hb :=
+  unfold access_heap in Hb; simpl in Hb;
+  try rewrite N.eqb_refl in Hb; simpl;
+  destruct_match; try discriminate;
+  try (rewrite decode_encode_int in Hb);
+  try rewrite <- Hb; destruct_match; inversion 1.
+
+Ltac forward_rg :=
+  let h := fresh "h" in
+  let h' := fresh "h" in
+  let p := fresh "p" in
+  let Hb := fresh "Hb" in
+  let HG := fresh "HG" in
+  apply RgStep;
+  intros h h' p Hb.
+
+Lemma inv_t1 : forall h bloc cloc (bal : Int),
+    let bm := MkMV bloc in
+    let cm := MkMV cloc in
+    access_heap h bloc = Some bal ->
+    bal >= 1000 ->
+    h ⊨ {{ R1 bloc }} (t1 bm cm) {{ G1 bloc }}.
+Proof.
+  intros.
+  unfold R1, G1.
+  
+  forward_rg.
+  rewrite H in Hb.
+  use_rely Hb.
+  split_g.
+  
+  forward_rg.
+  use_rely Hb0.
+  split_g.
+
+  forward_rg.
+  use_rely Hb1.
+  split_g.
+
+  forward_rg.
+  use_rely Hb2.
+  split_g.
+
+  forward_rg.
+  use_rely Hb3.
+  split_g.
+
+  forward_rg.
+  use_rely Hb4.
+  split_g.
+
+  eapply RgFinished. simpl.
+  intros. intuition.
+  unfold Int in H17.
+  rewrite <- H17 in H20. unfold access_heap in H20.
+  simpl in H20. rewrite N.eqb_refl in H20.
+  rewrite decode_encode_int in H20. inversion H20.
+  lia.
 Qed.
